```
1. (0, 5), (2,9)
   5 = a.0 + b
   9 = a.2 + b

   5 = b

   2a + 5 = 9
   2a = 9 - 5
   2a = 4
   a = 4 / 2
   a = 2

   f(x) =  2x + 5
---------------------
2. (1, 4), (3, 10)
   
   a = (y2 - y1) / (x2 - x1)

   a = (10 - 4) / (3 - 1)
   a = 6 / 2
   a = 3

   3.1 + b = 4
   b = 4 - 3
   b = 1

   f(x) = 3x + 1
---------------------
3. (0, -3), (4, 1)
   3 = a.0 + b
   1 = a.4 + b

   b = -3
   4a -3 = 1
   4a = 1 + 3
   4a = 4
   a = 4 / 4
   a = 1

   f(x) = 1x -3
---------------------
4. (-2, 8), (1, -1)
   8 = a.-2 + b
  -1 = a.1 + b

   a = (y2 - y1) / (x2 - x1)

   a = ((-1) - 8) / (1 - (-2))
   a = -9 / 3
   a = -3

   -3.(-2) + b = 8
   6 +  b = 8
   b = 8 - 6
   b = 2

   f(x) = -3x + 2
--------------------
5. (0, 2), (5, 2)
   2 = a.0 + b
   2 = a.5 + b

   b = 2
   5a + 2 = 2

   5a + 2 = 2
   5a = 2 - 2
   5a = 0
   a = 0 / 5
   a = 0

   f(x) = 0x + 2
```
